template-coq/src/quoter.ml
@@ -12,7 +12,7 @@ let cast_prop = ref (false)
 let is_cast_prop () = !cast_prop
 
 
-let toDecl (old: Name.t * ((Constr.constr) option) * Constr.constr) : Constr.rel_declaration =
+let toDecl (old: Name.t Context.binder_annot * ((Constr.constr) option) * Constr.constr) : Constr.rel_declaration =
   let (name,value,typ) = old in
   match value with
   | Some value -> Context.Rel.Declaration.LocalDef (name,value,typ)
@@ -60,15 +60,16 @@ sig
   val quote_variance : Univ.Variance.t -> quoted_variance
   val quote_abstract_univ_context : Univ.AUContext.t -> quoted_abstract_univ_context
 
+  val mkMonomorphic_entry : quoted_univ_contextset -> quoted_universes_entry
+  val mkPolymorphic_entry : quoted_name list -> quoted_univ_context -> quoted_universes_entry
+
   val mkMonomorphic_ctx : quoted_univ_contextset -> quoted_universes_decl
   val mkPolymorphic_ctx : quoted_abstract_univ_context -> quoted_universes_decl
-  val mkCumulative_ctx : quoted_abstract_univ_context -> quoted_variance list -> quoted_universes_decl
 
-  val quote_mind_params : (quoted_ident * (t,t) sum) list -> quoted_mind_params
   val quote_mind_finiteness : Declarations.recursivity_kind -> quoted_mind_finiteness
   val quote_mutual_inductive_entry :
-    quoted_mind_finiteness * quoted_mind_params * quoted_ind_entry list *
-    quoted_universes_decl ->
+    quoted_mind_finiteness * quoted_context (* params *) * quoted_ind_entry list *
+    quoted_universes_entry ->
     quoted_mind_entry
 
   val quote_entry : (quoted_definition_entry, quoted_mind_entry) sum option -> quoted_entry
@@ -87,6 +88,7 @@ sig
     -> quoted_context (* parameters context with lets *)
     -> quoted_one_inductive_body list
     -> quoted_universes_decl
+    -> quoted_variance list option
     -> quoted_mutual_inductive_body
 
   val mk_constant_body : t (* type *) -> t option (* body *) -> quoted_universes_decl -> quoted_constant_body
@@ -117,48 +119,42 @@ struct
   let push_rel decl (in_prop, env) = (in_prop, Environ.push_rel decl env)
   let push_rel_context ctx (in_prop, env) = (in_prop, Environ.push_rel_context ctx env)
 
-  (* From printmod.ml *)
-  let aucontext_ucontext univs =
-    let open Univ in
-    let inst = AUContext.instance univs in
-    let cst = UContext.constraints (AUContext.repr univs) in
-    (* let cst = AUContext.instantiate inst univs in *)
-    UContext.make (inst, cst)
-
   let get_abstract_inductive_universes iu =
     match iu with
-    | Declarations.Monomorphic_ind ctx -> Univ.ContextSet.to_context ctx
-    | Polymorphic_ind ctx -> Univ.AUContext.repr ctx
-    | Cumulative_ind cumi ->
-       (* let cumi = instantiate_cumulativity_info cumi in *)
-      Univ.AUContext.repr (Univ.ACumulativityInfo.univ_context cumi)  (* FIXME check also *)
+    | Declarations.Monomorphic ctx -> Univ.ContextSet.to_context ctx
+    | Polymorphic ctx -> Univ.AUContext.repr ctx
 
-  let quote_constant_uctx = function
-    | Monomorphic_const ctx -> Q.mkMonomorphic_ctx (Q.quote_univ_contextset ctx)
-    | Polymorphic_const ctx -> Q.mkPolymorphic_ctx (Q.quote_abstract_univ_context ctx)
+  let quote_universes_entry = function
+    | Monomorphic_entry ctx -> Q.mkMonomorphic_entry (Q.quote_univ_contextset ctx)
+    | Polymorphic_entry (names, ctx) -> 
+      Q.mkPolymorphic_entry (CArray.map_to_list Q.quote_name names) (Q.quote_univ_context ctx)
 
-  let quote_declarations_inductive_universes iu =
-    match iu with
-    | Monomorphic_ind ctx -> Q.mkMonomorphic_ctx (Q.quote_univ_contextset ctx)
-    | Polymorphic_ind ctx -> Q.mkPolymorphic_ctx (Q.quote_abstract_univ_context ctx)
-    | Cumulative_ind cumi ->
-      (* let cumi = instantiate_cumulativity_info cumi in *)
-      let ctx = Q.quote_abstract_univ_context (Univ.ACumulativityInfo.univ_context cumi) in
-      let var = CArray.map_to_list Q.quote_variance (Univ.ACumulativityInfo.variance cumi) in
-      Q.mkCumulative_ctx ctx var
-
-  let quote_entries_inductive_universes iu =
-    match iu with
-    | Monomorphic_ind_entry ctx -> Q.mkMonomorphic_ctx (Q.quote_univ_contextset ctx)
-    (* | Polymorphic_ind_entry ctx -> Q.mkPolymorphic_ctx (Q.quote_univ_context ctx)
-     * | Cumulative_ind_entry cumi ->
-     *   (\* let cumi = instantiate_cumulativity_info cumi in *\)
-     *   (\* FIXME variance is thrown away *\)
-     *    Q.mkCumulative_ctx (Q.quote_abstract_univ_context (Univ.ACumulativityInfo.univ_context cumi)) *)
-    | _ -> failwith "todo sim"
+  let quote_universes_decl = function
+    | Monomorphic ctx -> Q.mkMonomorphic_ctx (Q.quote_univ_contextset ctx)
+    | Polymorphic ctx -> Q.mkPolymorphic_ctx (Q.quote_abstract_univ_context ctx)
 
   let quote_inductive' (ind, i) =
     Q.quote_inductive (Q.quote_kn (Names.MutInd.canonical ind), Q.quote_int i)
+    
+  let quote_rel_decl quote_term acc env = function
+      | Context.Rel.Declaration.LocalAssum (na, t) ->
+        let t', acc = quote_term acc env t in
+        (Q.quote_context_decl (Q.quote_name (Context.binder_name na)) None t', acc)
+      | Context.Rel.Declaration.LocalDef (na, b, t) ->
+        let b', acc = quote_term acc env b in
+        let t', acc = quote_term acc env t in
+        (Q.quote_context_decl (Q.quote_name (Context.binder_name na)) (Some b') t', acc)
+  
+  let quote_rel_context quote_term acc env ctx =
+      let decls, env, acc =
+        List.fold_right (fun decl (ds, env, acc) ->
+            let x, acc = quote_rel_decl quote_term acc env decl in
+            (x :: ds, push_rel decl env, acc))
+          ctx ([],env,acc) in
+      Q.quote_context decls, acc
+
+  let quote_binder b = 
+    Q.quote_name (Context.binder_name b)
 
   let quote_term_remember
       (add_constant : KerName.t -> 'a -> 'a)
@@ -166,49 +162,50 @@ struct
     let rec quote_term (acc : 'a) env trm =
       let aux acc env trm =
       match Constr.kind trm with
-	Constr.Rel i -> (Q.mkRel (Q.quote_int (i - 1)), acc)
+	    | Constr.Rel i -> (Q.mkRel (Q.quote_int (i - 1)), acc)
       | Constr.Var v -> (Q.mkVar (Q.quote_ident v), acc)
       | Constr.Evar (n,args) ->
-	let (acc,args') =
-	  CArray.fold_left_map (fun acc x ->
-	    let (x,acc) = quote_term acc env x in acc,x)
-	                  acc args in
+	      let (acc,args') =
+      	  CArray.fold_left_map (fun acc x ->
+	        let (x,acc) = quote_term acc env x in acc,x)
+          acc args 
+        in
          (Q.mkEvar (Q.quote_int (Evar.repr n)) args', acc)
       | Constr.Sort s -> (Q.mkSort (Q.quote_sort s), acc)
       | Constr.Cast (c,k,t) ->
-	let (c',acc) = quote_term acc env c in
-	let (t',acc) = quote_term acc env t in
+	      let (c',acc) = quote_term acc env c in
+	      let (t',acc) = quote_term acc env t in
         let k' = Q.quote_cast_kind k in
         (Q.mkCast c' k' t', acc)
 
       | Constr.Prod (n,t,b) ->
-	let (t',acc) = quote_term acc env t in
+	      let (t',acc) = quote_term acc env t in
         let env = push_rel (toDecl (n, None, t)) env in
         let (b',acc) = quote_term acc env b in
-        (Q.mkProd (Q.quote_name n) t' b', acc)
+        (Q.mkProd (Q.quote_name (Context.binder_name n)) t' b', acc)
 
       | Constr.Lambda (n,t,b) ->
-	let (t',acc) = quote_term acc env t in
+	      let (t',acc) = quote_term acc env t in
         let (b',acc) = quote_term acc (push_rel (toDecl (n, None, t)) env) b in
-        (Q.mkLambda (Q.quote_name n) t' b', acc)
+        (Q.mkLambda (Q.quote_name (Context.binder_name n)) t' b', acc)
 
       | Constr.LetIn (n,e,t,b) ->
-	let (e',acc) = quote_term acc env e in
-	let (t',acc) = quote_term acc env t in
-	let (b',acc) = quote_term acc (push_rel (toDecl (n, Some e, t)) env) b in
-	(Q.mkLetIn (Q.quote_name n) e' t' b', acc)
+	      let (e',acc) = quote_term acc env e in
+	      let (t',acc) = quote_term acc env t in
+	      let (b',acc) = quote_term acc (push_rel (toDecl (n, Some e, t)) env) b in
+      	(Q.mkLetIn (Q.quote_name (Context.binder_name n)) e' t' b', acc)
 
       | Constr.App (f,xs) ->
-	let (f',acc) = quote_term acc env f in
-	let (acc,xs') =
-	  CArray.fold_left_map (fun acc x ->
-	    let (x,acc) = quote_term acc env x in acc,x)
-	    acc xs in
-	(Q.mkApp f' xs', acc)
+        let (f',acc) = quote_term acc env f in
+        let (acc,xs') =
+          CArray.fold_left_map (fun acc x ->
+            let (x,acc) = quote_term acc env x in acc,x)
+            acc xs in
+        (Q.mkApp f' xs', acc)
 
       | Constr.Const (c,pu) ->
          let kn = Names.Constant.canonical c in
-	 (Q.mkConst (Q.quote_kn kn) (Q.quote_univ_instance pu),
+	       (Q.mkConst (Q.quote_kn kn) (Q.quote_univ_instance pu),
           add_constant kn acc)
 
       | Constr.Construct ((mind,c),pu) ->
@@ -224,7 +221,7 @@ struct
                                       Q.quote_int (snd ci.Constr.ci_ind)) in
          let npar = Q.quote_int ci.Constr.ci_npar in
          let (qtypeInfo,acc) = quote_term acc env typeInfo in
-	 let (qdiscriminant,acc) = quote_term acc env discriminant in
+	       let (qdiscriminant,acc) = quote_term acc env discriminant in
          let (branches,nargs,acc) =
            CArray.fold_left2 (fun (xs,nargs,acc) x narg ->
                let (x,acc) = quote_term acc env x in
@@ -240,10 +237,10 @@ struct
          let pars = Q.quote_int (Projection.npars p) in
          let arg  = Q.quote_int (Projection.arg p)   in
          let p' = Q.quote_proj ind pars arg in
-         let kn = Names.Constant.canonical (Names.Projection.constant p) in
          let t', acc = quote_term acc env c in
          (Q.mkProj p' t', add_inductive (Projection.inductive p) acc)
       | Constr.Meta _ -> failwith "Meta not supported by TemplateCoq"
+      | Constr.Int _ -> failwith "Native integers not supported by TemplateCoq"
       in
       let in_prop, env' = env in
       if is_cast_prop () && not in_prop then
@@ -272,7 +269,7 @@ struct
       let ctxt =
         CArray.map2_i (fun i na t -> (Context.Rel.Declaration.LocalAssum (na, Vars.lift i t))) ns ts in
       let envfix = push_rel_context (CArray.rev_to_list ctxt) env in
-      let ns' = Array.map Q.quote_name ns in
+      let ns' = Array.map quote_binder ns in
       let b' = Q.quote_int b in
       let acc, ts' =
         CArray.fold_left_map (fun acc t -> let x,acc = quote_term acc env t in acc, x) acc ts in
@@ -286,21 +283,6 @@ struct
     and quote_cofixpoint acc env (a,decl) =
       let (a',decl'),acc = quote_recdecl acc env a decl in
       (Q.mkCoFix (a',decl'), acc)
-    and quote_rel_decl acc env = function
-      | Context.Rel.Declaration.LocalAssum (na, t) ->
-        let t', acc = quote_term acc env t in
-        (Q.quote_context_decl (Q.quote_name na) None t', acc)
-      | Context.Rel.Declaration.LocalDef (na, b, t) ->
-        let b', acc = quote_term acc env b in
-        let t', acc = quote_term acc env t in
-        (Q.quote_context_decl (Q.quote_name na) (Some b') t', acc)
-    and quote_rel_context acc env ctx =
-      let decls, env, acc =
-        List.fold_right (fun decl (ds, env, acc) ->
-            let x, acc = quote_rel_decl acc env decl in
-            (x :: ds, push_rel decl env, acc))
-          ctx ([],env,acc) in
-      Q.quote_context decls, acc
     and quote_minductive_type (acc : 'a) env (t : MutInd.t) =
       let mib = Environ.lookup_mind t (snd env) in
       let uctx = get_abstract_inductive_universes mib.Declarations.mind_universes in
@@ -308,7 +290,7 @@ struct
       let indtys =
         (CArray.map_to_list (fun oib ->
            let ty = Inductive.type_of_inductive (snd env) ((mib,oib),inst) in
-           (Context.Rel.Declaration.LocalAssum (Names.Name oib.mind_typename, ty))) mib.mind_packets)
+           (Context.Rel.Declaration.LocalAssum (Context.annotR (Names.Name oib.mind_typename), ty))) mib.mind_packets)
       in
       let envind = push_rel_context (List.rev indtys) env in
       let ref_name = Q.quote_kn (MutInd.canonical t) in
@@ -333,11 +315,11 @@ struct
 	  in
           let projs, acc =
             match mib.Declarations.mind_record with
-            | PrimRecord [|id, csts, ps|] ->  (* TODO handle mutual records *)
+            | PrimRecord [|id, csts, relevance, ps|] ->  (* TODO handle mutual records *)
                let ctxwolet = Termops.smash_rel_context mib.mind_params_ctxt in
                let indty = Constr.mkApp (Constr.mkIndU ((t,0),inst),
                                        Context.Rel.to_extended_vect Constr.mkRel 0 ctxwolet) in
-               let indbinder = Context.Rel.Declaration.LocalAssum (Names.Name id,indty) in
+               let indbinder = Context.Rel.Declaration.LocalAssum (Context.annotR (Names.Name id),indty) in
                let envpars = push_rel_context (indbinder :: ctxwolet) env in
                let ps, acc = CArray.fold_right2 (fun cst pb (ls,acc) ->
                  let (ty, acc) = quote_term acc envpars pb in
@@ -351,11 +333,12 @@ struct
 	  ([],acc) (Array.to_list mib.mind_packets)
       in
       let nparams = Q.quote_int mib.Declarations.mind_nparams in
-      let paramsctx, acc = quote_rel_context acc env mib.Declarations.mind_params_ctxt in
-      let uctx = quote_declarations_inductive_universes mib.Declarations.mind_universes in
+      let paramsctx, acc = quote_rel_context quote_term acc env mib.Declarations.mind_params_ctxt in
+      let uctx = quote_universes_decl mib.Declarations.mind_universes in
+      let var = Option.map (CArray.map_to_list Q.quote_variance) mib.Declarations.mind_variance in
       let bodies = List.map Q.mk_one_inductive_body (List.rev ls) in
       let finite = Q.quote_mind_finiteness mib.Declarations.mind_finite in
-      let mind = Q.mk_mutual_inductive_body finite nparams paramsctx bodies uctx in
+      let mind = Q.mk_mutual_inductive_body finite nparams paramsctx bodies uctx var in
       ref_name, Q.mk_inductive_decl mind, acc
     in ((fun acc env -> quote_term acc (false, env)),
         (fun acc env -> quote_minductive_type acc (false, env)))
@@ -397,10 +380,11 @@ struct
 	else
 	  begin
 	    visited_terms := Names.KNset.add kn !visited_terms ;
-            let c = Names.Constant.make kn kn in
+      let c = Names.Constant.make kn kn in
 	    let cd = Environ.lookup_constant c env in
-            let body = match cd.const_body with
-	      | Undef _ -> None
+      let body = match cd.const_body with
+        | Undef _ -> None
+        | Primitive _ -> CErrors.user_err Pp.(str "Primitives are unsupported by TemplateCoq")
 	      | Def cs -> Some (Mod_subst.force_constr cs)
 	      | OpaqueDef lc -> Some (Opaqueproof.force_proof (Global.opaque_tables ()) lc)
             in
@@ -413,7 +397,7 @@ struct
                              Feedback.msg_debug (str"Exception raised while checking body of " ++ KerName.print kn);
                  raise e
             in
-            let uctx = quote_constant_uctx cd.const_universes in
+            let uctx = quote_universes_decl cd.const_universes in
             let ty, acc =
               let ty = cd.const_type
                          (*CHANGE :  template polymorphism for definitions was removed.
@@ -448,6 +432,9 @@ struct
     let decls =  List.fold_left (fun acc (kn, d) -> Q.add_global_decl kn d acc) (Q.empty_global_declarations ()) !constants in
     Q.mk_program decls tm
 
+  let quote_rel_context env ctx = 
+    fst (quote_rel_context (fun acc env t -> (quote_term (snd env) t, acc)) () ((), env) ctx)
+
   let quote_one_ind envA envC (mi:Entries.one_inductive_entry) =
     let iname = Q.quote_ident mi.mind_entry_typename  in
     let arity = quote_term envA mi.mind_entry_arity in
@@ -456,32 +443,13 @@ struct
     let constypes = List.map (quote_term envC) (mi.mind_entry_lc) in
     (iname, arity, templatePoly, consnames, constypes)
 
-  let process_local_entry
-        (f: 'a -> Constr.t option (* body *) -> Constr.t (* type *) -> Names.Id.t -> Environ.env -> 'a)
-        ((env,a):(Environ.env*'a))
-        ((n,le):(Names.Id.t * Entries.local_entry))
-      :  (Environ.env * 'a) =
-    match le with
-    | Entries.LocalAssumEntry t -> (Environ.push_rel (toDecl (Names.Name n,None,t)) env, f a None t n env)
-    | Entries.LocalDefEntry b ->
-       let evm = Evd.from_env env in
-       let typ = EConstr.to_constr evm (Retyping.get_type_of env evm (EConstr.of_constr b)) in
-       (Environ.push_rel (toDecl (Names.Name n, Some b, typ)) env, f a (Some b) typ n env)
+  let quote_mind_params env (params: Constr.rel_context) =
+    let qparams = quote_rel_context env params in
+    (Environ.push_rel_context params env, qparams)
 
-  let quote_mind_params env (params:(Names.Id.t * Entries.local_entry) list) =
-    let f lr ob t n env =
-      match ob with
-      | Some b -> (Q.quote_ident n, Left (quote_term env b))::lr
-      | None ->
-         let t' = quote_term env t in
-         (Q.quote_ident n, Right t')::lr in
-    let (env, params) = List.fold_left (process_local_entry f) (env,[]) (List.rev params) in
-    (env, Q.quote_mind_params (List.rev params))
-
-  let mind_params_as_types ((env,t):Environ.env*Constr.t) (params:(Names.Id.t * Entries.local_entry) list) :
+  let mind_params_as_types ((env,t):Environ.env*Constr.t) (params:Constr.rel_context) :
         Environ.env*Constr.t =
-    List.fold_left (process_local_entry (fun tr ob typ n env -> Term.mkProd_or_LetIn (toDecl (Names.Name n,ob,typ)) tr)) (env,t)
-      (List.rev params)
+    (env, Term.it_mkProd_or_LetIn t params)
 
   (* CHANGE: this is the only way (ugly) I found to construct [absrt_info] with empty fields,
 since  [absrt_info] is a private type *)
@@ -498,12 +466,12 @@ since  [absrt_info] is a private type *)
                    snd (mind_params_as_types (env,x.mind_entry_arity) (t.mind_entry_params))))
         t.mind_entry_inds in
     (* env for quoting constructors of inductives. First push inductices, then params *)
-    let envC = List.fold_left (fun env p -> Environ.push_rel (toDecl (Names.Name (fst p), None, snd p)) env) env (one_arities) in
-    let (envC,_) = List.fold_left (process_local_entry (fun _ _ _ _ _ -> ())) (envC,()) (List.rev (t.mind_entry_params)) in
+    let envC = List.fold_left (fun env p -> Environ.push_rel (toDecl (Context.annotR (Names.Name (fst p)), None, snd p)) env) env (one_arities) in
+    let envC = Environ.push_rel_context t.mind_entry_params envC in
     (* env for quoting arities of inductives -- just push the params *)
-    let (envA,_) = List.fold_left (process_local_entry (fun _ _ _ _ _ -> ())) (env,()) (List.rev (t.mind_entry_params)) in
+    let envA = Environ.push_rel_context t.mind_entry_params env in
     let is = List.map (quote_one_ind envA envC) t.mind_entry_inds in
-   let uctx = quote_entries_inductive_universes t.mind_entry_universes in
+    let uctx = quote_universes_entry t.mind_entry_universes in
     Q.quote_mutual_inductive_entry (mf, mp, is, uctx)
 
   let quote_constant_body bypass env evm (cd : constant_body) =
@@ -516,9 +484,15 @@ since  [absrt_info] is a private type *)
         if bypass
         then Some (quote_term env (Opaqueproof.force_proof (Global.opaque_tables ()) cs))
         else None
+      | Primitive _ -> failwith "Primitive types not supported by TemplateCoq"
     in
-    let uctx = quote_constant_uctx cd.const_universes in
-    (ty, body, uctx)
+    let uctx = 
+      match cd.const_universes with
+      | Polymorphic auctx -> 
+        Polymorphic_entry (Univ.AUContext.names auctx, Univ.AUContext.repr auctx)
+      | Monomorphic ctx -> Monomorphic_entry ctx
+    in
+    (ty, body, quote_universes_entry uctx)
 
   let quote_entry_aux bypass env evm (name:string) =
     let (dp, nm) = split_name name in
