template-coq/theories/Constants.v
@@ -1,5 +1,5 @@
 From Coq Require Import Ascii String.
-From MetaCoq.Template Require Import BasicAst Ast utils.
+From MetaCoq.Template Require Import BasicAst Ast utils uGraph TemplateMonad TemplateMonad.Extractable.
 
 (* Base types *)
 
@@ -36,10 +36,198 @@ Register Coq.Init.Datatypes.inr as metacoq.sum.inr.
 Register Coq.Init.Datatypes.unit as metacoq.unit.type.
 Register Coq.Init.Datatypes.tt as metacoq.unit.intro.
 
+Register Coq.Init.Specif.sigT as metacoq.sigma.type.
+Register Coq.Init.Specif.existT as metacoq.sigma.intro.
+Register MetaCoq.Template.TemplateMonad.Common.existT_typed_term as metacoq.sigma.typed_term.
+
 (* Ast *)
 
 Register MetaCoq.Template.utils.NEL.sing as metacoq.nel.sing.
 Register MetaCoq.Template.utils.NEL.cons as metacoq.nel.cons.
 
-Register MetaCoq.BasicAst.nAnon as metacoq.ast.nAnon.
-Register MetaCoq.BasicAst.nNamed as metacoq.ast.nNamed.
+Register MetaCoq.Template.BasicAst.nAnon as metacoq.ast.nAnon.
+Register MetaCoq.Template.BasicAst.nNamed as metacoq.ast.nNamed.
+Register MetaCoq.Template.BasicAst.name as metacoq.ast.name.
+Register MetaCoq.Template.BasicAst.inductive as metacoq.ast.inductive.
+Register MetaCoq.Template.BasicAst.mkInd as metacoq.ast.mkInd.
+Register MetaCoq.Template.BasicAst.def as metacoq.ast.def.
+Register MetaCoq.Template.BasicAst.mkdef as metacoq.ast.mkdef.
+Register MetaCoq.Template.BasicAst.cast_kind as metacoq.ast.cast_kind.
+Register MetaCoq.Template.BasicAst.VmCast as metacoq.ast.VmCast.
+Register MetaCoq.Template.BasicAst.NativeCast as metacoq.ast.NativeCast.
+Register MetaCoq.Template.BasicAst.Cast as metacoq.ast.Cast.
+Register MetaCoq.Template.BasicAst.RevertCast as metacoq.ast.RevertCast.
+Register MetaCoq.Template.BasicAst.recursivity_kind as metacoq.ast.recursivity_kind.
+Register MetaCoq.Template.BasicAst.Finite as metacoq.ast.Finite.
+Register MetaCoq.Template.BasicAst.CoFinite as metacoq.ast.CoFinite.
+Register MetaCoq.Template.BasicAst.BiFinite as metacoq.ast.BiFinite.
+Register MetaCoq.Template.BasicAst.global_reference as metacoq.ast.global_reference.
+Register MetaCoq.Template.BasicAst.ConstRef as metacoq.ast.ConstRef.
+Register MetaCoq.Template.BasicAst.IndRef as metacoq.ast.IndRef.
+Register MetaCoq.Template.BasicAst.ConstructRef as metacoq.ast.ConstructRef.
+
+(* Universes *)
+
+Register MetaCoq.Template.Universes.sort_family as metacoq.ast.sort_family.
+Register MetaCoq.Template.Universes.fresh_level as metacoq.ast.fresh_level.
+Register MetaCoq.Template.Universes.fresh_universe as metacoq.ast.fresh_universe.
+Register MetaCoq.Template.Universes.InProp as metacoq.ast.InProp.
+Register MetaCoq.Template.Universes.InSet as metacoq.ast.InSet.
+Register MetaCoq.Template.Universes.InType as metacoq.ast.InType.
+Register MetaCoq.Template.Universes.ConstraintType.Le as metacoq.ast.constraints.Le.
+Register MetaCoq.Template.Universes.ConstraintType.Lt as metacoq.ast.constraints.Lt.
+Register MetaCoq.Template.Universes.ConstraintType.Eq as metacoq.ast.constraints.Eq.
+Register MetaCoq.Template.Universes.Universe.make'' as metacoq.ast.universe.make.
+Register MetaCoq.Template.Universes.LevelSetProp.of_list as metacoq.ast.universe.of_list.
+Register MetaCoq.Template.Universes.Level.t as metacoq.ast.level.t.
+Register MetaCoq.Template.Universes.Level.Level as metacoq.ast.level.Level.
+Register MetaCoq.Template.Universes.Level.lProp as metacoq.ast.level.lProp.
+Register MetaCoq.Template.Universes.Level.lSet as metacoq.ast.level.lSet.
+Register MetaCoq.Template.Universes.Level.Var as metacoq.ast.level.Var.
+
+Register MetaCoq.Template.Universes.Variance.t as metacoq.ast.variance.t.
+Register MetaCoq.Template.Universes.Variance.Irrelevant as metacoq.ast.variance.Irrelevant.
+Register MetaCoq.Template.Universes.Variance.Covariant as metacoq.ast.variance.Covariant.
+Register MetaCoq.Template.Universes.Variance.Invariant as metacoq.ast.variance.Invariant.
+
+Register MetaCoq.Template.Universes.universes_decl as metacoq.ast.universes_decl.
+Register MetaCoq.Template.Universes.Monomorphic_ctx as metacoq.ast.Monomorphic_ctx.
+Register MetaCoq.Template.Universes.Polymorphic_ctx as metacoq.ast.Polymorphic_ctx.
+
+Register MetaCoq.Template.Universes.ConstraintSet.t_ as metacoq.ast.ConstraintSet.t_.
+Register MetaCoq.Template.Universes.ConstraintSet.empty as metacoq.ast.ConstraintSet.empty.
+Register MetaCoq.Template.Universes.ConstraintSet.add as metacoq.ast.ConstraintSet.add.
+
+Register MetaCoq.Template.Universes.UContext.t as metacoq.ast.UContext.t.
+Register MetaCoq.Template.Universes.UContext.make as metacoq.ast.UContext.make.
+Register MetaCoq.Template.Universes.AUContext.t as metacoq.ast.AUContext.t.
+Register MetaCoq.Template.Universes.AUContext.make as metacoq.ast.AUContext.make.
+
+Register MetaCoq.Template.Universes.LevelSet.t_ as metacoq.ast.LevelSet.t.
+Register MetaCoq.Template.Universes.make_univ_constraint as metacoq.ast.make_univ_constraint.
+
+Register MetaCoq.Template.common.uGraph.init_graph as metacoq.ast.graph.init.
+(* FIXME wrong! *)
+Register MetaCoq.Template.common.uGraph.gc_of_constraints as metacoq.ast.graph.add_global_constraints.
+
+(* Terms *)
+
+Register MetaCoq.Template.Ast.term as metacoq.ast.term.
+Register MetaCoq.Template.Ast.tRel as metacoq.ast.tRel.
+Register MetaCoq.Template.Ast.tVar as metacoq.ast.tVar.
+Register MetaCoq.Template.Ast.tEvar as metacoq.ast.tEvar.
+Register MetaCoq.Template.Ast.tSort as metacoq.ast.tSort.
+Register MetaCoq.Template.Ast.tCast as metacoq.ast.tCast.
+Register MetaCoq.Template.Ast.tProd as metacoq.ast.tProd.
+Register MetaCoq.Template.Ast.tLambda as metacoq.ast.tLambda.
+Register MetaCoq.Template.Ast.tLetIn as metacoq.ast.tLetIn.
+Register MetaCoq.Template.Ast.tApp as metacoq.ast.tApp.
+Register MetaCoq.Template.Ast.tConst as metacoq.ast.tConst.
+Register MetaCoq.Template.Ast.tInd as metacoq.ast.tInd.
+Register MetaCoq.Template.Ast.tConstruct as metacoq.ast.tConstruct.
+Register MetaCoq.Template.Ast.tCase as metacoq.ast.tCase.
+Register MetaCoq.Template.Ast.tProj as metacoq.ast.tProj.
+Register MetaCoq.Template.Ast.tFix as metacoq.ast.tFix.
+Register MetaCoq.Template.Ast.tCoFix as metacoq.ast.tCoFix.
+
+(* Local and global declarations *)
+Register MetaCoq.Template.Ast.parameter_entry as metacoq.ast.parameter_entry.
+Register MetaCoq.Template.Ast.Build_parameter_entry as metacoq.ast.Build_parameter_entry.
+Register MetaCoq.Template.Ast.definition_entry as metacoq.ast.definition_entry.
+Register MetaCoq.Template.Ast.Build_definition_entry as metacoq.ast.Build_definition_entry.
+
+Register MetaCoq.Template.Universes.Monomorphic_ctx as metacoq.ast.Monomorphic_entry.
+Register MetaCoq.Template.Universes.Polymorphic_ctx as metacoq.ast.Polymorphic_entry.
+
+Register MetaCoq.Template.Ast.constant_entry as metacoq.ast.constant_entry.
+Register MetaCoq.Template.Ast.ParameterEntry as metacoq.ast.ParameterEntry.
+Register MetaCoq.Template.Ast.DefinitionEntry as metacoq.ast.DefinitionEntry.
+
+Register MetaCoq.Template.Ast.local_entry as metacoq.ast.local_entry.
+Register MetaCoq.Template.Ast.LocalDef as metacoq.ast.LocalDef.
+Register MetaCoq.Template.Ast.LocalAssum as metacoq.ast.LocalAssum.
+
+Register MetaCoq.Template.Ast.one_inductive_entry as metacoq.ast.one_inductive_entry.
+Register MetaCoq.Template.Ast.Build_one_inductive_entry as metacoq.ast.Build_one_inductive_entry.
+Register MetaCoq.Template.Ast.mutual_inductive_entry as metacoq.ast.mutual_inductive_entry.
+Register MetaCoq.Template.Ast.Build_mutual_inductive_entry as metacoq.ast.Build_mutual_inductive_entry.
+
+Register MetaCoq.Template.Ast.context_decl as metacoq.ast.context_decl.
+Register MetaCoq.Template.Ast.context as metacoq.ast.context.
+
+Register MetaCoq.Template.Ast.one_inductive_body as metacoq.ast.one_inductive_body.
+Register MetaCoq.Template.Ast.Build_one_inductive_body as metacoq.ast.Build_one_inductive_body.
+Register MetaCoq.Template.Ast.mutual_inductive_body as metacoq.ast.mutual_inductive_body.
+Register MetaCoq.Template.Ast.Build_mutual_inductive_body as metacoq.ast.Build_mutual_inductive_body.
+Register MetaCoq.Template.Ast.constant_body as metacoq.ast.constant_body.
+Register MetaCoq.Template.Ast.constant_body as metacoq.ast.Build_constant_body.
+
+Register MetaCoq.Template.Ast.global_decl as metacoq.ast.global_decl.
+Register MetaCoq.Template.Ast.ConstantDecl as metacoq.ast.ConstantDecl.
+Register MetaCoq.Template.Ast.InductiveDecl as metacoq.ast.InductiveDecl.
+Register MetaCoq.Template.Ast.global_env as metacoq.ast.global_env.
+Register MetaCoq.Template.Ast.global_env_ext as metacoq.ast.global_env_ext.
+Register MetaCoq.Template.Ast.program as metacoq.ast.program.
+
+(* Template monad *)
+
+Register MetaCoq.Template.TemplateMonad.Common.cbv as metacoq.template.cbv.
+Register MetaCoq.Template.TemplateMonad.Common.cbn as metacoq.template.cbn.
+Register MetaCoq.Template.TemplateMonad.Common.hnf as metacoq.template.hnf.
+Register MetaCoq.Template.TemplateMonad.Common.all as metacoq.template.all.
+Register MetaCoq.Template.TemplateMonad.Common.lazy as metacoq.template.lazy.
+Register MetaCoq.Template.TemplateMonad.Common.unfold as metacoq.template.unfold.
+
+(* Prop *)
+Register MetaCoq.Template.TemplateMonad.Core.tmReturn as metacoq.templatemonad.prop.tmReturn.
+Register MetaCoq.Template.TemplateMonad.Core.tmBind as metacoq.templatemonad.prop.tmBind.
+Register MetaCoq.Template.TemplateMonad.Core.tmPrint as metacoq.templatemonad.prop.tmPrint.
+Register MetaCoq.Template.TemplateMonad.Core.tmMsg as metacoq.templatemonad.prop.tmMsg.
+Register MetaCoq.Template.TemplateMonad.Core.tmFail as metacoq.templatemonad.prop.tmFail.
+Register MetaCoq.Template.TemplateMonad.Core.tmEval as metacoq.templatemonad.prop.tmEval.
+Register MetaCoq.Template.TemplateMonad.Core.tmLemma as metacoq.templatemonad.prop.tmLemma.
+Register MetaCoq.Template.TemplateMonad.Core.tmDefinitionRed_ as metacoq.templatemonad.prop.tmDefinitionRed_.
+Register MetaCoq.Template.TemplateMonad.Core.tmAxiomRed as metacoq.templatemonad.prop.tmAxiomRed.
+Register MetaCoq.Template.TemplateMonad.Core.tmMkDefinition as metacoq.templatemonad.prop.tmMkDefinition.
+Register MetaCoq.Template.TemplateMonad.Core.tmMkInductive as metacoq.templatemonad.prop.tmMkInductive.
+Register MetaCoq.Template.TemplateMonad.Core.tmFreshName as metacoq.templatemonad.prop.tmFreshName.
+Register MetaCoq.Template.TemplateMonad.Core.tmAbout as metacoq.templatemonad.prop.tmAbout.
+Register MetaCoq.Template.TemplateMonad.Core.tmCurrentModPath as metacoq.templatemonad.prop.tmCurrentModPath.
+
+Register MetaCoq.Template.TemplateMonad.Core.tmQuote as metacoq.templatemonad.prop.tmQuote.
+Register MetaCoq.Template.TemplateMonad.Core.tmQuoteRec as metacoq.templatemonad.prop.tmQuoteRec.
+Register MetaCoq.Template.TemplateMonad.Core.tmQuoteInductive as metacoq.templatemonad.prop.tmQuoteInductive.
+Register MetaCoq.Template.TemplateMonad.Core.tmQuoteConstant as metacoq.templatemonad.prop.tmQuoteConstant.
+Register MetaCoq.Template.TemplateMonad.Core.tmQuoteUniverses as metacoq.templatemonad.prop.tmQuoteUniverses.
+
+Register MetaCoq.Template.TemplateMonad.Core.tmUnquote as metacoq.templatemonad.prop.tmUnquote.
+Register MetaCoq.Template.TemplateMonad.Core.tmUnquoteTyped as metacoq.templatemonad.prop.tmUnquoteTyped.
+
+Register MetaCoq.Template.TemplateMonad.Core.tmInferInstance as metacoq.templatemonad.prop.tmInferInstance.
+Register MetaCoq.Template.TemplateMonad.Core.tmExistingInstance as metacoq.templatemonad.prop.tmExistingInstance.
+
+Register MetaCoq.Template.TemplateMonad.Core.tmTestQuote as metacoq.templatemonad.prop.tmTestQuote.
+Register MetaCoq.Template.TemplateMonad.Core.tmQuoteDefinition as metacoq.templatemonad.prop.tmQuoteDefinition.
+Register MetaCoq.Template.TemplateMonad.Core.tmQuoteDefinitionRed as metacoq.templatemonad.prop.tmQuoteDefinitionRed.
+Register MetaCoq.Template.TemplateMonad.Core.tmQuoteRecDefinition as metacoq.templatemonad.prop.tmQuoteRecDefinition.
+
+
+(* Type *)
+Register MetaCoq.Template.TemplateMonad.Extractable.tmReturn as metacoq.templatemonad.type.tmReturn.
+Register MetaCoq.Template.TemplateMonad.Extractable.tmBind as metacoq.templatemonad.type.tmBind.
+Register MetaCoq.Template.TemplateMonad.Extractable.tmPrint as metacoq.templatemonad.type.tmPrint.
+Register MetaCoq.Template.TemplateMonad.Extractable.tmMsg as metacoq.templatemonad.type.tmMsg.
+Register MetaCoq.Template.TemplateMonad.Extractable.tmFail as metacoq.templatemonad.type.tmFail.
+Register MetaCoq.Template.TemplateMonad.Extractable.tmEval as metacoq.templatemonad.type.tmEval.
+Register MetaCoq.Template.TemplateMonad.Extractable.tmDefinition_ as metacoq.templatemonad.type.tmDefinition_.
+Register MetaCoq.Template.TemplateMonad.Extractable.tmAxiom as metacoq.templatemonad.type.tmAxiom.
+Register MetaCoq.Template.TemplateMonad.Extractable.tmLemma as metacoq.templatemonad.type.tmLemma.
+Register MetaCoq.Template.TemplateMonad.Extractable.tmFreshName as metacoq.templatemonad.type.tmFreshName.
+Register MetaCoq.Template.TemplateMonad.Extractable.tmAbout as metacoq.templatemonad.type.tmAbout.
+Register MetaCoq.Template.TemplateMonad.Extractable.tmCurrentModPath as metacoq.templatemonad.type.tmCurrentModPath.
+Register MetaCoq.Template.TemplateMonad.Extractable.tmQuoteInductive as metacoq.templatemonad.type.tmQuoteInductive.
+Register MetaCoq.Template.TemplateMonad.Extractable.tmQuoteUniverses as metacoq.templatemonad.type.tmQuoteUniverses.
+Register MetaCoq.Template.TemplateMonad.Extractable.tmQuoteConstant as metacoq.templatemonad.type.tmQuoteConstant.
+Register MetaCoq.Template.TemplateMonad.Extractable.tmInductive as metacoq.templatemonad.type.tmInductive.
+Register MetaCoq.Template.TemplateMonad.Extractable.tmInferInstance as metacoq.templatemonad.type.tmInferInstance.
+Register MetaCoq.Template.TemplateMonad.Extractable.tmExistingInstance as metacoq.templatemonad.type.tmExistingInstance.
